expand RVShadowStackProperties, bugfix in stack

examples/rv/RVShadowStackProperties.v
@@ -2,6 +2,9 @@
 Require Import Koika.BitsToLists Koika.Frontend Koika.UntypedIndSemantics.
 Require Import rv.Stack rv.RVCore rv.rv32 rv.rv32i.
 
+Import Coq.Lists.List.ListNotations.
+Scheme Equality for list.
+
 (* We mostly reason on the instruction that is currently entering the execute
    stage. All the information available about it is in the d2e structure
    (decode to execute buffer). *)
@@ -9,13 +12,15 @@ Section ShadowStackProperties.
   Context {REnv : Env RV32I.reg_t}.
   Definition schedule := rv_schedule.
 
+  Definition eql (l1 l2: list bool) : bool := list_beq bool Bool.eqb l1 l2.
+
   (* Propositions about the initial state *)
   Definition no_mispred
     (ctx: env_t REnv (fun _ : RV32I.reg_t => BitsToLists.val))
   : Prop :=
     forall v,
     getenv REnv ctx (RV32I.d2e (RV32I.fromDecode.data0)) =
-      Struct (RV32I.decode_bookkeeping) v ->
+      Struct (RV32I.decode_bookkeeping) v /\
     get_field_struct (struct_fields RV32I.decode_bookkeeping) v "epoch" =
     Some (getenv REnv ctx (RV32I.epoch)).
 
@@ -34,13 +39,89 @@ Section ShadowStackProperties.
       (bits_t RV32I.Stack.index_sz)
       (Bits.of_nat (RV32I.Stack.index_sz) RV32I.Stack.capacity).
 
-  (* Definition is_call_instruction (instr: bits_t 32) := *)
-  (* Definition is_ret_instruction (instr: bits_t 32):=. *)
+  (* XXX Note that both a pop and a push can happen for the same instruction *)
 
-  (* Definition stack_push := is_call_instruction (). *)
-  (* Definition stack_pop := is_ret_instruction (). *)
+  (* This function is defined in a way that mirrors RVCore.v *)
+  Definition is_call_instruction (instr: bits_t 32) : bool :=
+    let bits := vect_to_list (bits_of_value instr) in
+    let opcode_ctrl := List.firstn 3 (List.skipn 4 bits) in
+    let opcode_rest := List.firstn 4 (List.skipn 0 bits) in
+    let rs1 := List.firstn 5 (List.skipn 15 bits) in
+    let rd := List.firstn 5 (List.skipn 7 bits) in
+    (eql opcode_ctrl [true; true; false])
+    && (
+      (
+        (eql opcode_rest [true; true; true; true])
+        && (
+          (eql rd [false; false; false; false; true])
+          || (eql rd [false; false; true; false; true])
+        )
+      )
+      || (
+        (eql opcode_rest [false; true; true; true])
+        && (
+          (eql rd [false; false; false; false; true])
+          || (eql rd [false; false; true; false; true])
+        )
+      )
+    ).
 
-  (* TODO should never return None, simplify *)
+  (* This function is defined in a way that mirrors RVCore.v *)
+  Definition is_ret_instruction (instr: bits_t 32) : bool :=
+    let bits := vect_to_list (bits_of_value instr) in
+    let opcode_ctrl := List.firstn 3 (List.skipn 4 bits) in
+    let opcode_rest := List.firstn 4 (List.skipn 0 bits) in
+    let rs1 := List.firstn 5 (List.skipn 15 bits) in
+    let rd := List.firstn 5 (List.skipn 7 bits) in
+    (eql opcode_ctrl [true; true; false])
+    && (eql opcode_rest [false; true; true; true])
+    && (
+      (
+        (
+          (eql rd [false; false; false; false; true])
+          || (eql rd [false; false; true; false; true])
+        )
+        && (negb (eql rd rs1))
+        && (
+          (eql rs1 [false; false; false; false; true])
+          || (eql rs1 [false; false; true; false; true])
+        )
+      )
+      || (
+        (negb (eql rd [false; false; false; false; true]))
+        && (eql rd [false; false; true; false; true])
+        && (
+          (eql rs1 [false; false; false; false; true])
+          || (eql rs1 [false; false; true; false; true])
+        )
+      )
+    ).
+
+  Definition stack_push
+    (ctx: env_t REnv (fun _ : RV32I.reg_t => BitsToLists.val))
+  : Prop :=
+    forall v w b,
+    getenv REnv ctx (RV32I.d2e (RV32I.fromDecode.data0)) =
+      Struct (RV32I.decode_bookkeeping) v /\
+    get_field_struct (struct_fields RV32I.decode_bookkeeping) v "dInst" =
+      Some (Struct (decoded_sig) w) /\
+    get_field_struct (struct_fields decoded_sig) w "inst" =
+      Some (Bits 32 b) /\
+    is_call_instruction (Bits.of_N 32 (Bits.to_N (vect_of_list b))) = true.
+
+  Definition stack_pop
+    (ctx: env_t REnv (fun _ : RV32I.reg_t => BitsToLists.val))
+  : Prop :=
+    forall v w b,
+    getenv REnv ctx (RV32I.d2e (RV32I.fromDecode.data0)) =
+      Struct (RV32I.decode_bookkeeping) v /\
+    get_field_struct (struct_fields RV32I.decode_bookkeeping) v "dInst" =
+      Some (Struct (decoded_sig) w) /\
+    get_field_struct (struct_fields decoded_sig) w "inst" =
+      Some (Bits 32 b) /\
+    is_ret_instruction (Bits.of_N 32 (Bits.to_N (vect_of_list b))) = true.
+
+  (* TODO should never return None, simplify? *)
   Definition stack_push_address
     (ctx: env_t REnv (fun _ : RV32I.reg_t => BitsToLists.val))
   : option (bits_t 32) :=
@@ -60,39 +141,37 @@ Section ShadowStackProperties.
     | _ => None
     end.
 
+  (* TODO should never return None, simplify? *)
   Definition stack_top_address
     (ctx: env_t REnv (fun _ : RV32I.reg_t => BitsToLists.val))
   : option (bits_t 32) :=
-    let index := getenv REnv ctx (RV32I.stack RV32I.Stack.size) in
-    let data := getenv REnv ctx (RV32I.stack RV32I.Stack.stack).
-
-    (* forall (ctx: env_t REnv (fun _ : RV32I.reg_t => BitsToLists.val)) v,*)
-    (* getenv REnv ctx (RV32I.d2e (RV32I.fromDecode.data0)) =*)
-    (*   Struct (RV32I.decode_bookkeeping) v*)
-    (* -> get_field_struct (struct_fields RV32I.decode_bookkeeping) v "dInst"*)
-    (*   = Some (Bits 32 [*)
-    (*     false; false; false; false; false; false; false; false; false; false;*)
-    (*     false; false; false; false; false; false; false; false; false; false;*)
-    (*     false; false; false; false; false; false; false; false; false; false;*)
-    (*     false; false*)
-    (*     ]). *)
+    let index_raw := getenv REnv ctx (RV32I.stack RV32I.Stack.size) in
+    let index_nat := Bits.to_nat (vect_of_list (ubits_of_value index_raw)) in
+    let index := index_of_nat (pow2 RV32I.Stack.index_sz) index_nat in
+    match index with
+    | Some x =>
+      let data_raw := (getenv REnv ctx (RV32I.stack (RV32I.Stack.stack x))) in
+      Some (Bits.of_N 32 (Bits.to_N (vect_of_list (ubits_of_value data_raw))))
+    | None => None
+    end.
 
   Definition stack_underflow
     (ctx: env_t REnv (fun _ : RV32I.reg_t => BitsToLists.val))
-  : Prop := no_mispred ctx && stack_empty ctx && stack_pop ctx.
+  : Prop := no_mispred ctx /\ stack_empty ctx /\ stack_pop ctx.
   Definition stack_overflow
     (ctx: env_t REnv (fun _ : RV32I.reg_t => BitsToLists.val))
-  : Prop := no_mispred ctx && stack_full ctx && stack_push ctx.
+  : Prop :=
+    no_mispred ctx /\ stack_full ctx /\ (not (stack_pop ctx)) /\ stack_push ctx.
   Definition stack_address_violation
     (ctx: env_t REnv (fun _ : RV32I.reg_t => BitsToLists.val))
   : Prop := forall x y,
-    no_mispred ctx && stack_push ctx && stack_top_address ctx = x
-    && stack_push_address ctx = y && x <> y.
+    no_mispred ctx /\ stack_push ctx /\ stack_top_address ctx = x
+    /\ stack_push_address ctx = y /\ x <> y.
 
   Definition stack_violation
     (ctx: env_t REnv (fun _ : RV32I.reg_t => BitsToLists.val))
   : Prop :=
-    stack_underflow ctx || stack_overflow ctx || stack_address_violation ctx.
+    stack_underflow ctx \/ stack_overflow ctx \/ stack_address_violation ctx.
 
   (* Final state *)
   Definition halt_set := .
@@ -122,8 +201,8 @@ Section ShadowStackProperties.
 
   (* Main theorem *)
   Theorem shadow_stack_ok:
-    halt_leads_to_a_sink_state && stack_violation_results_in_halt
-    && no_stack_violation_behaves_as_if_no_stack.
+    halt_leads_to_a_sink_state /\ stack_violation_results_in_halt
+    /\ no_stack_violation_behaves_as_if_no_stack.
   Proof.
   Qed.
 End ShadowStackProperties.
